\begin{array}{c} \begin{array}{l} \left(\left(\sum_{i=2}^{4} \left(\left(i \cdot \left(i + 1\right)\right) \cdot \left(x {\otimes} y\right)\right)\right) \in \left(\mathbb{R}^{3} {\otimes} \mathbb{R}^{3}\right)\right) \\  \Rightarrow \left(\begin{array}{c} \begin{array}{l} \left(\left(\gamma \cdot \beta\right) \cdot \left(\sum_{i=2}^{4} \left(\left(i \cdot \left(i + 1\right)\right) \cdot \left(x {\otimes} y\right)\right)\right)\right) \\  = \left(\sum_{i=2}^{4} \left(\left(\left(\gamma \cdot \beta\right) \cdot \left(i \cdot \left(i + 1\right)\right)\right) \cdot \left(x {\otimes} y\right)\right)\right) \end{array} \end{array}\right) \end{array} \end{array}