\left(a_{1}, \ldots, a_{m}, b_{1}, \ldots, b_{n}, c, d_{1}, \ldots, d_{k}\right) \mapsto \left\{\# (a_{1} ~ \ldots ~ a_{m} ~ \left(b_{1} + \ldots + b_{n}\right) ~ d_{1} ~ \ldots ~ d_{k}) = \# (a_{1} ~ \ldots ~ a_{m} ~ c ~ d_{1} ~ \ldots ~ d_{k}) \textrm{ if } a_{1} \in \mathbb{N}^{\leq 9} ,  \ldots ,  a_{m} \in \mathbb{N}^{\leq 9} ,  b_{1} \in \mathbb{N}^{\leq 9} ,  \ldots ,  b_{n} \in \mathbb{N}^{\leq 9} ,  c \in \mathbb{N}^{\leq 9} ,  d_{1} \in \mathbb{N}^{\leq 9} ,  \ldots ,  d_{k} \in \mathbb{N}^{\leq 9} ,  \left(b_{1} + \ldots + b_{n}\right) = c\right..