\left(\forall_{a_{1}, b_{1}~|~a_{1} = b_{1}}~\left(\left(a_{1}\right) = \left(b_{1}\right)\right), \forall_{m \in \mathbb{N}^+~|~\forall_{a_{1}, a_{2}, \ldots, a_{m}, b_{1}, b_{2}, \ldots, b_{m}~|~\left(a_{1} = b_{1}\right), \left(a_{2} = b_{2}\right), \ldots, \left(a_{m} = b_{m}\right)}~\left(\left(a_{1}, a_{2}, \ldots, a_{m}\right) = \left(b_{1}, b_{2}, \ldots, b_{m}\right)\right)}~\left[\forall_{a_{1}, a_{2}, \ldots, a_{m + 1}, b_{1}, b_{2}, \ldots, b_{m + 1}~|~\left(a_{1} = b_{1}\right), \left(a_{2} = b_{2}\right), \ldots, \left(a_{m + 1} = b_{m + 1}\right)}~\left(\left(a_{1}, a_{2}, \ldots, a_{m + 1}\right) = \left(b_{1}, b_{2}, \ldots, b_{m + 1}\right)\right)\right]\right)