\left(\left(\sum_{i=2}^{4} \left(x {\otimes} y {\otimes} f\left(i\right) {\otimes} z\right)\right) \in \left(\mathbb{R}^{3} {\otimes} \mathbb{R}^{3} {\otimes} \mathbb{R}^{3} {\otimes} \mathbb{R}^{3}\right), \begin{array}{c} \begin{array}{l} \left(\gamma \cdot \left(\sum_{i=2}^{4} \left(x {\otimes} y {\otimes} f\left(i\right) {\otimes} z\right)\right)\right) \\  = \left(\sum_{i=2}^{4} \left(\gamma \cdot \left(x {\otimes} y {\otimes} f\left(i\right) {\otimes} z\right)\right)\right) \end{array} \end{array}\right)