\begin{array}{c} \begin{array}{l} \left[\forall_{i \in \{2~\ldotp \ldotp~4\}}~\left(\left(x {\otimes} f\left(i\right) {\otimes} y\right) \in \left(\mathbb{R}^{3} {\otimes} \mathbb{R}^{3} {\otimes} \mathbb{R}^{3}\right)\right)\right] \Rightarrow  \\ \left(\begin{array}{c} \begin{array}{l} \left(x {\otimes} \left(\sum_{i=2}^{4} f\left(i\right)\right) {\otimes} y\right) \\  = \left(\sum_{i=2}^{4} \left(x {\otimes} f\left(i\right) {\otimes} y\right)\right) \end{array} \end{array}\right) \end{array} \end{array}