\left(A, B\right) \mapsto \left\{\begin{array}{c} \begin{array}{l} \left(\left[A, B\right] = \vec{0}\left(\mathcal{L}\left(\mathcal{H}, \mathcal{H}\right)\right)\right) \Leftrightarrow  \\ \left[\begin{array}{l}\exists_{x_{1}, x_{2}, \ldots, x_{n}~|~\left\{x_{1}, x_{2}, \ldots, x_{n}\right\} \in \textrm{O.N.Bases}\left(\mathcal{H}\right)}~\\
\left[\begin{array}{l}\exists_{a_{1}, a_{2}, \ldots, a_{n}, b_{1}, b_{2}, \ldots, b_{n} \in \mathbb{C}}~\\
\left(\begin{array}{c} \left(A = \left(\sum_{i=1}^{n} \left(a_{i} \cdot \textrm{OrthoProj}\left(\mathcal{H}, \textrm{Span}\left(\left\{x_{i}\right\}\right)\right)\right)\right)\right) \land  \\ \left(B = \left(\sum_{i=1}^{n} \left(b_{i} \cdot \textrm{OrthoProj}\left(\mathcal{H}, \textrm{Span}\left(\left\{x_{i}\right\}\right)\right)\right)\right)\right) \end{array}\right)\end{array}\right]\end{array}\right] \end{array} \end{array} \textrm{ if } A \in \mathcal{L}\left(\mathcal{H}, \mathcal{H}\right) ,  B \in \mathcal{L}\left(\mathcal{H}, \mathcal{H}\right) ,  A^{\dagger} = A ,  B^{\dagger} = B\right..