\left(|\left((\lnot B_{1}), (\lnot B_{2}), \ldots, (\lnot B_{i - 1}),C_{1}, C_{2}, \ldots, C_{i}, A \lor D\right)| = |\left(1, 2, \ldots, m\right)|, \left(1, 2, \ldots, \left(i - 1\right),i, \left(i + 1\right), \ldots, j, m\right) = \left(1, 2, \ldots, m\right), |\left((\lnot B_{1}), (\lnot B_{2}), \ldots, (\lnot B_{i - 1})\right)| = |\left(1, 2, \ldots, \left(i - 1\right)\right)|, |\left(C_{1}, C_{2}, \ldots, C_{i}\right)| = |\left(i, \left(i + 1\right), \ldots, j\right)|, \left(1, 2, \ldots, j, m\right) = \left(1, 2, \ldots, m\right), |\left((\lnot B_{1}), (\lnot B_{2}), \ldots, (\lnot B_{i - 1}),C_{1}, C_{2}, \ldots, C_{i}\right)| = |\left(1, 2, \ldots, j\right)|\right)