\left\{\begin{array}{c} \left(A_{1} \land \ldots \land A_{l} \land B \land C_{1} \land \ldots \land C_{m} \land D_{1} \land \ldots \land D_{n}\right) =  \\ \left(A_{1} \land \ldots \land A_{l} \land C_{1} \land \ldots \land C_{m} \land B \land D_{1} \land \ldots \land D_{n}\right) \end{array} \textrm{ if } A_{1} \in \mathbb{B} ,  \ldots ,  A_{l} \in \mathbb{B} ,  B \in \mathbb{B} ,  C_{1} \in \mathbb{B} ,  \ldots ,  C_{m} \in \mathbb{B} ,  D_{1} \in \mathbb{B} ,  \ldots ,  D_{n} \in \mathbb{B}\right..