\left(\begin{array}{c} \left[\forall_{a_{1}, b_{1}~|~a_{1} = b_{1}}~\left(\left(a_{1}\right) = \left(b_{1}\right)\right)\right] \\  \land \left[\forall_{m \in \mathbb{N}^+~|~\forall_{a_{1}, \ldots, a_{m}, b_{1}, \ldots, b_{m}~|~a_{1} = b_{1}, \ldots, a_{m} = b_{m}}~\left(\left(a_{1}, \ldots, a_{m}\right) = \left(b_{1}, \ldots, b_{m}\right)\right)}~\left[\forall_{a_{1}, \ldots, a_{m + 1}, b_{1}, \ldots, b_{m + 1}~|~a_{1} = b_{1}, \ldots, a_{m + 1} = b_{m + 1}}~\left(\left(a_{1}, \ldots, a_{m + 1}\right) = \left(b_{1}, \ldots, b_{m + 1}\right)\right)\right]\right] \end{array}, \forall_{n \in \mathbb{N}^+}~\left[\forall_{a_{1}, \ldots, a_{n}, b_{1}, \ldots, b_{n}~|~a_{1} = b_{1}, \ldots, a_{n} = b_{n}}~\left(\left(a_{1}, \ldots, a_{n}\right) = \left(b_{1}, \ldots, b_{n}\right)\right)\right]\right)