\begin{array}{c} \begin{array}{l} \left[\forall_{i \in \{2~\ldotp \ldotp~4\}}~\left(\left(\gamma \cdot \beta \cdot i \cdot \left(i + 1\right)\right) = \left(\left(\gamma \cdot \beta\right) \cdot i \cdot \left(i + 1\right)\right)\right)\right] \Rightarrow  \\ \left(\begin{array}{c} \begin{array}{l} \left[i \mapsto \left\{\gamma \cdot \beta \cdot i \cdot \left(i + 1\right) \textrm{ if } i \in \{2~\ldotp \ldotp~4\}\right..\right] =  \\ \left[i \mapsto \left\{\left(\gamma \cdot \beta\right) \cdot i \cdot \left(i + 1\right) \textrm{ if } i \in \{2~\ldotp \ldotp~4\}\right..\right] \end{array} \end{array}\right) \end{array} \end{array}